Proved erasure for the new kind of safety.

concurrency/concurrent_machine.v
@@ -13,6 +13,8 @@ Require Import concurrency.addressFiniteMap.
 Require Import concurrency.scheduler.
 Require Import Coq.Program.Program.
 
+Require Import concurrency.safety.
+
 (* This module represents the arguments
    to build a CoreSemantics with 
    compcert mem. This is used by BOTH
@@ -494,7 +496,7 @@ Module CoarseMachine (SCH:Scheduler)(SIG : ConcurrentMachineSig with Module Thre
         (Hcmpt: mem_compatible ms m)
         (Htstep: threadStep genv Htid Hcmpt ms' m' ev),
         machine_step U [::] ms m U [::] ms' m'
-  | suspend_step: (*Want to remove*)
+  | suspend_step:
       forall tid U U' ms ms' m
         (HschedN: schedPeek U = Some tid)
         (HschedS: schedSkip U = U')        (*Schedule Forward*)
@@ -601,6 +603,82 @@ Module CoarseMachine (SCH:Scheduler)(SIG : ConcurrentMachineSig with Module Thre
                  (Hstep: MachStep ge st m (schedSkip (fst (fst st)),[::],tp') m')
                  (Hsafe: forall U'', csafe ge (U'',[::],tp') m' n),
       csafe ge st m (S n).
+
+  Section new_safety.
+  (** *I create a new type of safety that satisfies (forall n, safeN) -> safe and is preserved by simulations. *)
+    
+    Inductive sem_with_halt ge: MachState -> mem -> MachState -> mem -> Prop:=
+    | halt_with_step st m: halted st -> sem_with_halt ge st m st m
+    | step_with_halt st m st' m' : MachStep ge st m st' m' -> sem_with_halt ge st m st' m'.
+    
+  Definition new_state: Type:= seq machine_event * machine_state * mem.
+  Definition mk_nstate (st:MachState) m:new_state:= (snd (fst st), snd st, m).
+  Definition mk_ostate (st:new_state) U:MachState:= (U, fst (fst st), snd (fst st)).
+  Definition new_step ge (st: new_state) U st' U': Prop:=
+    sem_with_halt ge (mk_ostate st U) (snd st) (mk_ostate st' U') (snd st').
+  (*This has to be filled in:*)
+  Axiom valid: MachState -> bool.
+  Definition new_valid st U := valid (mk_ostate st U). 
+  Definition ksafe_new_step (ge : G) (st : MachState) (m : mem) : nat -> Prop :=
+    ksafe _ _ (new_step ge) new_valid (mk_nstate st m) (fst (fst st)).
+
+  (*Things that we must prove:*)
+  Axiom sch_dec: forall (U U': Sch), {U = U'} + {U <> U'}.
+  Axiom step_sch: forall {ge U tr tp m U' tr' tp' m'}, MachStep ge (U, tr, tp) m (U', tr', tp') m' -> {U=U'}+{schedSkip(U)=U'}.
+  Axiom step_trace: forall {ge U tr tp m U' tr' tp' m'}, MachStep ge (U, tr, tp) m (U', tr', tp') m' -> nil = tr'. 
+  Axiom step_valid: forall {ge st m st' m'}, MachStep ge st m st' m'  -> valid st -> valid st'. 
+  Axiom step_sch_valid: forall {ge U tr tp m U' tr' tp' m'}, MachStep ge (U, tr, tp) m (U', tr', tp') m' -> U<>U' -> forall U'', valid (U'', tr', tp').
+  Axiom skip_not_eq: forall U, U <> schedSkip U.
+  Lemma safety_equivalence':
+    forall ge st_ m,
+      (forall U n, new_valid (nil, st_, m) U -> ksafe_new_step ge (U, nil, st_) m n) ->
+      (forall U n, valid (U, nil, st_) ->  csafe ge (U, nil, st_) m n).
+  Proof.
+    move=> ge st_ m KSF' U n VAL.
+    assert (KSF: forall U, new_valid (nil, st_, m) U -> ksafe_new_step ge (U, nil, st_) m n) by (move=> U'' NV; apply: KSF'=>// ).
+    clear KSF'.
+    assert (VAL_: new_valid (nil, st_, m) U) by rewrite /new_valid /mk_ostate /= //. clear VAL.
+    (*move: VAL_=> /(KSF _ n) KSF_new.*)
+    move: st_ m KSF U VAL_.
+    induction n.
+    - constructor.
+    - move => st_ m KSF U nVAL.
+      move: (nVAL) => /KSF => KSF_new.
+      inversion KSF_new; subst.
+      move: H0; rewrite /new_step /mk_nstate /= => STEP_halt.
+      inversion STEP_halt.
+      + subst; move: H6; rewrite /mk_ostate=> H6; apply: HaltedSafe=>//.
+      + subst; move: H; rewrite /mk_ostate /= => H.
+          assert (HH:=step_trace H); rewrite -HH in H.
+        destruct (step_sch H).
+        * subst U'; apply: (CoreSafe _ _ _ (snd (fst st')) (snd st')) =>/= //.
+          { apply: IHn => //.
+            - move => U'' nVAL'; rewrite /ksafe_new_step /mk_nstate => /=.
+              destruct st' as [p m0]; destruct p=> /=. simpl in HH; rewrite -HH in H1.
+              apply: H1=> //.
+            - rewrite /new_valid /mk_ostate=> /=.
+              apply: (step_valid H) =>//.
+          }
+        * subst U'. apply: (AngelSafe _ _ _ (snd (fst st')) (snd st'))=>//.
+          move=>U''.
+          { destruct st' as [[tr' tp'] m'] => /=; eapply IHn.
+            - move => U0 nVAL0. rewrite /ksafe_new_step /mk_nstate=> /=.
+              simpl in HH; rewrite -HH in H1.
+              by apply: H1. 
+            - rewrite /new_valid /mk_ostate=> /=. simpl in H.
+              apply (step_sch_valid H).
+                by apply: skip_not_eq.
+          }
+  Qed.
+        
+  Lemma safety_equivalence:
+    forall ge tp m,
+      (forall U, new_valid (nil, tp, m) U) ->
+      (forall n U, ksafe_new_step ge (U, nil, tp) m n) ->
+      (forall n U, csafe ge (U, nil, tp) m n).
+  Proof. by move => ? ? ? H ? ? ?; apply: safety_equivalence'; try apply: H. Qed.
+  
+  End new_safety.
 
   Lemma csafe_reduce:
     forall ge sched tp mem n m,
