concurrency/erasure_safety.v
@@ -58,9 +58,7 @@ Module ErasureSafety.
     induction n.
     intros. constructor.
     intros. inversion H1.
-(*    - (*Safe_0*) constructor.  *)
-    - (*HaltedSafe*)
-      constructor; simpl. unfold DryMachine.halted; simpl.
+    - constructor; simpl. unfold DryMachine.halted; simpl.
       unfold JuicyMachine.halted in H2; simpl in H2.
       change JuicyMachineModule.THE_JUICY_MACHINE.SCH.schedPeek with
       DryMachineSource.THE_DRY_MACHINE_SOURCE.SCH.schedPeek in H2.
@@ -116,5 +114,141 @@ Qed.
     as [mu [ds [_ [dinit [dinv MTCH]]]]]; eauto.
     unfold init_inj_ok; intros b b' ofs H. inversion H.
   Qed.
+
+  (** *Lets proof that again with the new kind of safety*)
+  Lemma new_erasure_safety'': forall n ge js ds m,
+      ErasureProof.match_st js ds ->
+      DSEM.invariant ds ->
+      (forall sch, JuicyMachine.valid (sch, nil, js) -> JuicyMachine.ksafe_new_step ge (sch, nil, js) m n) ->
+      (forall sch, DryMachine.valid (sch, nil, ds) -> DryMachine.ksafe_new_step ge (sch, nil, ds) m n).
+  Proof.
+    assert (assume: forall js ds, match_st js ds -> forall sch, JuicyMachine.valid (sch, nil, js) <-> DryMachine.valid (sch, nil, ds)) by admit.
+    induction n; [intros; constructor| ].
+    move => ge js ds m MATCH INV H1 sch VAL. specialize (H1 sch).
+    move: VAL (MATCH) => /assume /H1 HH /HH KSF.
+    inversion KSF.
+    rewrite /DryMachine.ksafe_new_step /DryMachine.mk_nstate /=.
+    move: H0; rewrite /JuicyMachine.new_step /JuicyMachine.mk_ostate /= => H3.
+    inversion H3.
+    { (*Halted case*)
+      destruct st as [[a b] c]; destruct st' as [[a' b'] c']; simpl in *.
+      inversion H4; subst.
+      apply: (safety.sft_step).
+      - apply: DryMachine.halt_with_step=> //. 
+      - move => U'' nVAL.
+        apply: IHn => //.
+        + apply: (MATCH).
+        + rewrite /JuicyMachine.ksafe_new_step /JuicyMachine.mk_nstate /=.
+          move=>sch' /assume JVAL; move: (MATCH) => /JVAL DVAL.
+          apply: H2.
+          rewrite /JuicyMachine.new_valid /JuicyMachine.mk_ostate /=.
+          move: DVAL MATCH => /assume KK /KK //.
+    }
+    { (* Step Case*)
+      assert (step_diagram:=step_diagram).
+      specialize (step_diagram m initU sch U' (Some init_rmap) (Some init_pmap)).
+      specialize (step_diagram ds js).
+      specialize (step_diagram (snd (fst st')) (snd st')).
+      unfold JuicyMachine.MachStep in step_diagram; simpl in step_diagram.
+      unfold JuicyMachineModule.THE_JUICY_MACHINE.JuicyMachine.MachStep in step_diagram; simpl in step_diagram.
+      destruct st as [[a b] c]; destruct st' as [[a' b'] c']; simpl in *.
+      inversion H4; subst.
+      (*We need to talk about traces... until now... they are empty:*)
+      assert (requirement:(a') = nil) by admit.
+      rewrite requirement in H0.
+      eapply step_diagram in H0 => //.
+      destruct H0 as [ ds' [ Dinv' [ match' step']]].
+      apply: (safety.sft_step).
+        - by eapply (DryMachine.step_with_halt _ _ _ (DryMachine.mk_ostate (nil, ds', c') U')) => //.
+        - (*rewrite /JuicyMachine.ksafe_new_step /JuicyMachine.mk_nstate /=.
+          move=>sch' /assume /= JVAL'. move: (match') => /JVAL' JVAL.
+          rewrite requirement in H2.*)
+          move => U'' nVAL.
+          apply: IHn => //.
+          + exact match'.
+          + rewrite /JuicyMachine.ksafe_new_step /JuicyMachine.mk_nstate /=.
+          move=>sch' /assume JVAL; move: (match') => /JVAL DVAL.
+          rewrite requirement in H2; apply: H2.
+          rewrite /JuicyMachine.new_valid /JuicyMachine.mk_ostate /=.
+          move: DVAL match' => /assume KK /KK //.
+    }
+  Admitted.
+
+  Lemma new_erasure_safety': forall n ge sch js ds m,
+      ErasureProof.match_st js ds ->
+      DSEM.invariant ds ->
+      JuicyMachine.ksafe_new_step ge (sch, nil, js) m n ->
+      DryMachine.ksafe_new_step ge (sch, nil, ds) m n.
+  Proof.
+    induction n; [intros; constructor| ].
+    intros. inversion H1.
+    rewrite /DryMachine.ksafe_new_step /DryMachine.mk_nstate /=.
+    move: H3; rewrite /JuicyMachine.new_step /JuicyMachine.mk_ostate /==> HH.
+    inversion HH.
+    { (*Halted case*)
+      apply: (safety.sft_step).
+      - apply: DryMachine.halt_with_step=> //. 
+      - move => U'' nVAL.
+        apply: IHn => //.
+        + apply: H.
+        + rewrite /JuicyMachine.ksafe_new_step /JuicyMachine.mk_nstate /=.
+          destruct st' as [[a b] c]/ ; subst=> /=.
+          simpl in H8; rewrite -H8 in H4.
+          apply: H4.
+          simpl in nVAL.
+        subst.
+    }
+    {  assert (step_diagram:=step_diagram).
+        specialize (step_diagram m initU sch U' (Some init_rmap) (Some init_pmap)).
+        specialize (step_diagram ds js).
+        specialize (step_diagram (snd (fst st')) (snd st')).
+        unfold JuicyMachine.MachStep in step_diagram; simpl in step_diagram.
+        unfold JuicyMachineModule.THE_JUICY_MACHINE.JuicyMachine.MachStep in step_diagram; simpl in step_diagram.
+        assert (requirement:(fst (fst st')) = nil) by admit.
+        rewrite requirement in H3.
+        eapply step_diagram in H3 => //.
+        destruct H3 as [ ds' [ Dinv' [ match' step']]].
+
+        apply: (safety.sft_step).
+        - by eapply (DryMachine.step_with_halt _ _ _ (DryMachine.mk_ostate (nil, ds', (snd st')) U')) => //.
+        - move => U''
+        
+        rewrite requirement.
+        apply step'.
+        (*Halted case: *)
+        
+        
+      unfold corestep in step_diagram; simpl in step_diagram.
+      
+    - apply: (safety.sft_step ) => //.
+      simpl in H3; inversion H3.
+      
+
+      constructor; simpl. unfold DryMachine.halted; simpl.
+      unfold JuicyMachine.halted in H2; simpl in H2.
+      change JuicyMachineModule.THE_JUICY_MACHINE.SCH.schedPeek with
+      DryMachineSource.THE_DRY_MACHINE_SOURCE.SCH.schedPeek in H2.
+      destruct ( DryMachineSource.THE_DRY_MACHINE_SOURCE.SCH.schedPeek sch ) eqn:AA;
+      inversion H; auto.
+    - { simpl in Hstep.
+        unfold JuicyMachine.MachStep in Hstep; simpl in Hstep.
+        assert (step_diagram:=step_diagram).
+        specialize (step_diagram m initU sch sch (Some init_rmap) (Some init_pmap)).
+        specialize (step_diagram ds js tp' m').
+        unfold corestep in step_diagram; simpl in step_diagram.
+        unfold JuicyMachine.MachStep in step_diagram; simpl in step_diagram.
+        eapply step_diagram in Hstep; try eassumption.
+        destruct Hstep as [ds' [dinv' [MATCH' stp']]].
+        econstructor 3; eauto. }
+    - { simpl in Hstep.
+        unfold JuicyMachine.MachStep in Hstep; simpl in Hstep.
+        assert (step_diagram:=step_diagram).
+        specialize (step_diagram m initU sch (SCH.schedSkip sch) (Some init_rmap) (Some init_pmap)).
+        specialize (step_diagram ds js tp' m').
+        unfold corestep in step_diagram; simpl in step_diagram.
+        unfold JuicyMachine.MachStep in step_diagram; simpl in step_diagram.
+        eapply step_diagram in Hstep; try eassumption.
+        destruct Hstep as [ds' [dinv' [MATCH' stp']]].
+        econstructor 4; eauto. }
     
 End ErasureSafety. 
